work

src/Lean/Meta/Tactic/Rfl.lean
@@ -8,7 +8,9 @@ module
 prelude
 public import Lean.Elab.Tactic.Basic
 public import Lean.Meta.Tactic.Refl
--- public import Lean.Meta.Tactic.Relations
+public import Lean.Meta.Tactic.Relations
+public import Lean.Meta.Tactic.Replace
+public import Lean.Meta.CongrTheorems
 
 public section
 
@@ -21,7 +23,7 @@ provided the reflexivity lemma has been marked as `@[refl]`.
 
 namespace Lean.Meta.Rfl
 
-open Lean Meta
+open Lean Meta Elab Tactic
 
 /-- Environment extensions for `refl` lemmas -/
 initialize reflExt :
@@ -31,33 +33,140 @@ initialize reflExt :
     initial := {}
   }
 
+/-- Returns the refl lemmas that match the given relation. -/
+def getReflLemmas (rel : Expr) : MetaM (Array Name) := do
+  (reflExt.getState (← getEnv)).getMatch rel
+
 /--
 Tags reflexivity lemmas to be used by the `rfl` tactic.
 
 A reflexivity lemma should have the conclusion `r x x` where `r` is an arbitrary relation.
 
-It is not allowed to tag reflexivity lemmas for `=` using this attribute. These are handled as a
+Tagging reflexivity lemmas for `=` is not allowed using this attribute. These are handled as a
 special case in the `rfl` tactic.
+
+Relations can be declared first using the `@[relation]` attribute, which may be necessary
+if the left-hand, but `@[refl]` will
 -/
 @[builtin_doc]
 builtin_initialize registerBuiltinAttribute {
   name := `refl
-  descr := "reflexivity relation"
+  descr := "reflexivity lemma for a relation"
   add := fun decl _ kind => MetaM.run' do
-    let declTy := (← getConstInfo decl).type
-    let (_, _, targetTy) ← withReducible <| forallMetaTelescopeReducing declTy
-    let fail := throwError
-      "`[refl]` attribute only applies to lemmas of the form `x ∼ x`, but this declaration is not:\
-        {inlineExprTrailing declTy}"
-    let .app (.app rel lhs) rhs ← whnfCore targetTy | fail
-    if let .app (.const ``Eq [_]) _ := rel then
-      throwError "`[refl]` attribute may not be used on `Eq.refl`"
-    unless ← withNewMCtxDepth <| isDefEq lhs rhs do fail
-    let key ← DiscrTree.mkPath rel
-    reflExt.add (decl, key) kind
+    withTraceNode `Meta.Tactic.relation (fun _ => return m!"adding [refl] lemma `{.ofConstName decl}`") do
+      let declTy := (← getConstInfo decl).type
+      forallTelescope declTy fun _ targetTy => do
+        let targetTy ← whnfCore targetTy
+        let .const relName _ := targetTy.getAppFn
+          | throwError "\
+              `[refl]` attribute only applies to lemmas concluding with `x ∼ x`, where the relation is \
+              a constant application, but the conclusion is not a constant application:\
+              {inlineExprTrailing targetTy}"
+        if relName == ``Eq then
+          throwError "`[refl]` attribute may not be used on `Eq`"
+        -- If the this isn't a registered relation, automatically infer and register it.
+        if (← getRelationInfo? relName).isNone then
+          withTraceNode `Meta.Tactic.relation (fun _ => return m!"Unknown relation, inferring [relation] for `{.ofConstName relName}`.") do
+            let info ← inferRelationInfo relName #[]
+            registerRelation relName info kind
+        let some info ← matchesRelation? targetTy | unreachable!
+        -- Validate the conclusion of the lemma
+        unless ← withNewMCtxDepth <| isDefEq info.lhs info.rhs do
+          let (lhs, rhs) ← addPPExplicitToExposeDiff info.lhs info.rhs
+          throwError "\
+            `[refl]` attribute only applies to lemmas concluding with `x ∼ x`,
+            but the left-hand side{indentExpr lhs}\nis not definitionally equal to the right-hand side{indentExpr rhs}"
+        -- Validate applicability of the lemma
+        let g ← mkFreshExprSyntheticOpaqueMVar declTy
+        let gs ← g.mvarId!.apply (← mkConstWithFreshMVarLevels decl) (term? := m!"'{.ofConstName decl}'")
+        unless gs.isEmpty do
+          throwError "`[refl]` lemma cannot be applied, has unsolved goals\n{goalsToMessageData gs}"
+      let (_, _, targetTy) ← forallMetaTelescope declTy
+      let some info ← matchesRelation? (← whnfCore targetTy) | unreachable!
+      let key ← DiscrTree.mkPath info.rel
+      reflExt.add (decl, key) kind
 }
 
-open Elab Tactic
+private def throwNoRflLemma {α} (tacticName : Name) (goal : MVarId) (rel : Expr) : MetaM α :=
+  throwTacticEx tacticName goal <| m!"No `[refl]` lemma registered for relation{indentExpr rel}"
+    ++ MessageData.hint' m!"Add the `[refl]` attribute to reflexivity lemmas for{inlineExpr rel}to use this tactic"
+
+private def applyLemmas (tacticName : Name) (goal : MVarId) (rel : Expr) (lems : Array Name) : MetaM Unit := do
+  let mut ex? := none
+  let s ← saveState
+  for lem in lems do
+    try
+      let gs ← goal.apply (← mkConstWithFreshMVarLevels lem) (term? := m!"'{.ofConstName lem}'")
+      unless gs.isEmpty do
+        throwError MessageData.tagged `Tactic.unsolvedGoals <| m!"unsolved goals\n{goalsToMessageData gs}"
+      -- Success!
+      return ()
+    catch e =>
+      unless ex?.isSome do
+        ex? := some (← saveState, e) -- stash the first failure
+    s.restore
+  if let some (sErr, e) := ex? then
+    sErr.restore
+    throw e
+  else
+    s.restore
+    throwNoRflLemma tacticName goal rel
+
+/--
+Finds a `@[refl]` lemma that applies.
+The type `t` is defeq to the type of `goal`.
+Unfolds `t` step-by-step looking for lemmas.
+-/
+private partial def applyRflCore (goal : MVarId) (t : Expr) : MetaM Unit := do
+  let t ← whnfCore t
+  if !t.getAppFn.isConst then
+    throwRelError
+  else if t.isAppOfArity ``Eq 3 then
+    -- The common case is equality: just use `Eq.refl`
+    let_expr Eq α lhs rhs := t | unreachable!
+    checkDefEq lhs rhs
+    let us := t.getAppFn.constLevels!
+    goal.assign (mkApp2 (mkConst ``Eq.refl us) α lhs)
+  else if t.isAppOfArity ``HEq 4 then
+    -- `HEq` is less common, but we can give a more precise error report than for general relations
+    let_expr HEq α lhs β rhs := t | unreachable!
+    let us := t.getAppFn.constLevels!
+    checkDefEq α β "type"
+    checkDefEq lhs rhs
+    goal.assign (mkApp2 (mkConst ``HEq.refl us) α lhs)
+  else if t.isAppOfArity ``Iff 2 then
+    -- This is unnecessary, but it's a common case.
+    let_expr Iff lhs rhs := t | unreachable!
+    checkDefEq lhs rhs
+    goal.assign (mkApp (mkConst ``Iff.refl []) lhs)
+  else if let some info@{ rel, lhs, rhs, .. } ← matchesRelation? t then
+    -- Search through `[refl]` keyed by the relation
+    let lems ← getReflLemmas rel
+    if lems.isEmpty then
+      tryUnfold goal t (throwNoRflLemma `rfl goal rel)
+    else
+      checkDefEq lhs rhs
+      -- We change the type to `lhs ~ lhs` so that we don't do the (possibly costly) `lhs =?= rhs`
+      -- check again.
+      let t := t.withApp fun f args => mkAppN f (args.set! info.rhsIdx lhs)
+      goal.setType t
+      applyLemmas `rfl goal rel lems
+  else
+    tryUnfold goal t throwRelError
+where
+  throwRelError :=
+    throwTacticEx `rfl goal <| m!"Expecting a goal that is a binary relation"
+      ++ MessageData.hint' m!"Reflexivity tactics can only be used on goals of the form `x ~ x` or `R x x`"
+  checkDefEq (lhs rhs : Expr) (thing : MessageData := "side") := do
+    unless ← approxDefEq <| isDefEq lhs rhs do
+      throwTacticEx `rfl goal <| MessageData.ofLazyM (es := #[lhs, rhs]) do
+        let (lhs, rhs) ← addPPExplicitToExposeDiff lhs rhs
+        return m!"The left-hand {thing}{indentExpr lhs}\nis not definitionally equal to the right-hand {thing}{indentExpr rhs}"
+  tryUnfold (goal : MVarId) (t : Expr) (err : MetaM Unit) : MetaM Unit := do
+    if let some t' ← unfoldDefinition? t then
+      applyRflCore goal t'
+    else
+      err
 
 /-- `MetaM` version of the `rfl` tactic.
 
@@ -66,87 +175,155 @@ relation, that is, equality or another relation which has a reflexive lemma tagg
 attribute [refl].
 -/
 def _root_.Lean.MVarId.applyRfl (goal : MVarId) : MetaM Unit := goal.withContext do
-  -- NB: uses reducible whnf, we do not want to unfold the relation itself
-  let t ← withReducible goal.getType'
-  if t.getAppNumArgs < 2 then
-    throwTacticEx `rfl goal <| m!"Expected the goal to be a binary relation"
-      ++ MessageData.hint' m!"Reflexivity tactics can only be used on goals of the form `x ~ x` or `R x x`"
+  goal.checkNotAssigned `rfl
+  let t ← goal.getType
+  applyRflCore goal t {}
 
-  -- Special case HEq here as it has a different argument order.
-  if t.isAppOfArity ``HEq 4 then
-    let gs ← goal.applyConst ``HEq.refl
-    unless gs.isEmpty do
-      throwTacticEx `rfl goal <| MessageData.tagged `Tactic.unsolvedGoals <| m!"unsolved goals\n{
-        goalsToMessageData gs}"
-    return
+/--
+Finds a `@[refl]` lemma that applies to lift `x ~ y` to `x = y` or `x ≍ y`.
+The type `t` is defeq to the type of `goal`.
+Unfolds `t` step-by-step looking for lemmas.
 
-  let rel := t.appFn!.appFn!
-  let lhs := t.appFn!.appArg!
-  let rhs := t.appArg!
-
-  let success ← approxDefEq <| isDefEqGuarded lhs rhs
-  unless success do
-    let explanation := MessageData.ofLazyM (es := #[lhs, rhs]) do
-      let (lhs, rhs) ← addPPExplicitToExposeDiff lhs rhs
-      return m!"The left-hand side{indentExpr lhs}\nis not definitionally equal to the right-hand side{indentExpr rhs}"
-    throwTacticEx `rfl goal explanation
-
-  if rel.isAppOfArity `Eq 1 then
-    -- The common case is equality: just use `Eq.refl`
-    let us := rel.appFn!.constLevels!
-    let α :=  rel.appArg!
-    goal.assign (mkApp2 (mkConst ``Eq.refl us) α lhs)
-  else
-    -- Else search through `@refl` keyed by the relation
-    -- We change the type to `lhs ~ lhs` so that we don't do the (possibly costly) `lhs =?= rhs`
-    -- check again.
-    goal.setType (.app t.appFn! lhs)
-    let s ← saveState
-    let mut ex? := none
-    for lem in ← (reflExt.getState (← getEnv)).getMatch rel do
-      try
-        let gs ← goal.apply (← mkConstWithFreshMVarLevels lem) (term? := m!"'{.ofConstName lem}'")
-        if gs.isEmpty then return () else
-          throwError MessageData.tagged `Tactic.unsolvedGoals <| m!"unsolved goals\n{
-            goalsToMessageData gs}"
-      catch e =>
-        unless ex?.isSome do
-          ex? := some (← saveState, e) -- stash the first failure of `apply`
-      s.restore
-    if let some (sErr, e) := ex? then
-      sErr.restore
-      throw e
+This is a congruence task. The key problems are:
+1. Taking `x ~ y` and finding a way to turn it into `x ~ x` (the relation might be heterogeneous,
+   and there might be typeclass instances).
+2. Proving that `x = y → (x ~ x = x ~ y)`.
+-/
+private partial def liftReflToEqHEqCore (goal : MVarId) (t : Expr) (allowHEq : Bool := true) : MetaM MVarId := do
+  let t ← whnfCore t
+  if !t.getAppFn.isConst then
+    throwRelError
+  else if t.isAppOfArity ``Eq 3 then
+    -- Already Eq
+    goal.setType t
+    return goal
+  else if t.isAppOfArity ``HEq 4 then
+    -- Already HEq.
+    goal.setType t
+    let goal ← goal.heqOfEq
+    unless allowHEq do
+      if let some (lhsTy, _, rhsTy, _) := (← goal.getType).heq? then
+        throwTypeNotDefEqError lhsTy rhsTy
+    return goal
+  else if t.isAppOfArity ``Iff 2 then
+    -- There is a meta tactic for this, so may as well use it for this common case.
+    goal.setType t
+    goal.iffOfEq
+  else if let some info@{ rel, lhs, rhs, .. } ← matchesRelation? t then
+    -- Search through `[refl]` keyed by the relation
+    let lems ← getReflLemmas rel
+    if lems.isEmpty then
+      tryUnfold goal t (throwNoRflLemma rel)
     else
-      throwTacticEx `rfl goal <| m!"No `[refl]` lemma registered for relation{indentExpr rel}"
-        ++ MessageData.hint' m!"Add the `[refl]` attribute to reflexivity lemmas for{inlineExpr rel}to use this tactic"
-
-/-- Helper theorem for `Lean.MVarId.liftReflToEq`. -/
-theorem rel_of_eq_and_refl {α : Sort _} {R : α → α → Prop}
-    {x y : α} (hxy : x = y) (h : R x x) : R x y :=
-  hxy ▸ h
+      let lhsTy ← inferType lhs
+      let lhsU ← getLevel lhsTy
+      let rhsTy ← inferType rhs
+      let rhsU ← getLevel rhsTy
+      unless ← isLevelDefEq lhsU rhsU do
+        -- If the universe levels are different, then they can't be Eq or HEq.
+        throwTacticEx `liftReflToEq goal "The universe level of left-hand type{indentExpr lhsTy}\n\
+          is not definitionally equal to the universe level of right-hand type{indentExpr rhsTy}"
+      -- Try unifying the types
+      let typesEq ← approxDefEq <| isDefEq lhsTy rhsTy
+      if !allowHEq && !typesEq then
+        throwTypeNotDefEqError lhsTy rhsTy
+      if typesEq && info.rhsIdx == info.numArgs - 1 then
+        -- Common case: `Eq` where rhs is the last argument.
+        -- The `@[relation]` attribute validates that the type of the relation doesn't depend on the arguments
+        let goalEq ← mkFreshExprSyntheticOpaqueMVar (tag := ← goal.getTag) (← mkEq lhs rhs)
+        let pf ← mkCongrArg t.appFn! goalEq  -- Proof that `lhs ~ lhs = lhs ~ rhs`
+        let t' := Expr.app t.appFn! lhs
+        let goal' ← goal.replaceTargetEq t' (← mkEqSymm pf)
+        applyLemmas `liftReflToEq goal' rel lems
+        return goalEq.mvarId!
+      else
+        -- Otherwise, use a congruence lemma.
+        let congr ← mkHCongr rel
+        let throwCongrError {α} (_ : Unit) : MetaM α :=
+          throwTacticEx `liftReflToEq goal m!"Failed to construct equation to rewrite relation{indentExpr t}\nto be reflexive"
+        unless congr.argKinds[info.rhsIdx - info.relArgs]! matches .eq | .heq do
+          throwCongrError ()
+        let (args, _, teq) ← forallMetaTelescope congr.type
+        -- We're going for `teq : lhs ~ lhs = lhs ~ rhs`
+        -- This way, the congruence goal `goalEq` is `lhs = rhs` (or `lhs ≍ rhs`).
+        let some (_, trfl, t') := teq.eq? | throwCongrError ()
+        unless ← isDefEq t' t do throwCongrError ()  -- sets all arguments for `t` (*)
+        -- Locate where the arguments for each kind are in `args`
+        let (kindArgIdxs, _) := congr.argKinds.foldl (init := (#[], 0)) fun (kindArgIdxs, idx) kind =>
+          (kindArgIdxs.push idx,
+            match kind with
+            | .fixed | .cast    => idx + 1
+            | .subsingletonInst => idx + 2
+            | .eq | .heq        => idx + 3
+            | .fixedNoParam     => unreachable!)
+        -- Three arguments: trfl's lhs, t's lhs, and eq/heq. t's lhs already set at (*)
+        let lhsArgIdx := kindArgIdxs[info.lhsIdx - info.relArgs]!
+        -- Three arguments: trfl's rhs, t's rhs, and eq/heq. t's rhs already set at (*)
+        let rhsArgIdx := kindArgIdxs[info.rhsIdx - info.relArgs]! -- lhs =/≍ rhs
+        -- Set up `trfl` as `lhs ~ lhs`, and set the eq/heq for the lhs
+        unless ← approxDefEq <| isDefEq args[lhsArgIdx]! lhs do throwCongrError ()
+        try (← args[lhsArgIdx+2]!.mvarId!.heqOfEq).refl catch _ => throwCongrError ()
+        unless ← approxDefEq <| isDefEq args[rhsArgIdx]! lhs do throwCongrError ()
+        -- This is the goal we want to reduce the relation to:
+        let goalEq := args[rhsArgIdx+2]!.mvarId!
+        goalEq.setKind .syntheticOpaque
+        -- Reduce the main goal to proving reflexivity:
+        let goal ← goal.replaceTargetEq trfl (← mkEqSymm (mkAppN congr.proof args))
+        -- Apply reflexivity lemmas. This will also ensure remaining arguments are synthesized.
+        applyLemmas `liftReflToEq goal rel lems
+        -- Now prove remaining equality goals
+        let goalEq ← goalEq.heqOfEq
+        let mut unsolved := #[]
+        for kind in congr.argKinds, idx in kindArgIdxs do
+          if idx != rhsArgIdx && kind matches .eq | .heq then
+            let g ← pure args[idx+2]!.mvarId!
+            let g ← g.heqOfEq
+            try
+              g.refl
+                <|> do (guard <| ← g.subsingletonElim)
+                <|> do
+                      let pf ← mkAppM ``type_eq_of_heq #[.mvar goalEq]
+                      guard <| ← isDefEq (.mvar g) pf
+                      g.assign pf
+            catch _ =>
+              unsolved := unsolved.push g
+        unless unsolved.isEmpty do
+          throwError MessageData.tagged `Tactic.unsolvedGoals <| m!"unsolved goals\n{goalsToMessageData unsolved.toList}"
+        return goalEq
+  else
+    tryUnfold goal t throwRelError
+where
+  throwRelError :=
+    throwTacticEx `liftReflToEq goal <| m!"Expected the goal to be a binary relation"
+      ++ MessageData.hint' m!"Reflexivity tactics can only be used on goals of the form `x ~ y`"
+  throwNoRflLemma {α} (rel : Expr) : MetaM α :=
+    throwTacticEx `liftReflToEq goal <| m!"No `[refl]` lemma registered for relation{indentExpr rel}"
+      ++ MessageData.hint' m!"Add the `[refl]` attribute to reflexivity lemmas for{inlineExpr rel}to use this tactic"
+  throwTypeNotDefEqError (lhsTy rhsTy : Expr) :=
+    throwTacticEx `liftReflToEq goal <| MessageData.ofLazyM (es := #[lhsTy, rhsTy]) do
+      let (lhsTy, rhsTy) ← addPPExplicitToExposeDiff lhsTy rhsTy
+      return m!"The left-hand type{indentExpr lhsTy}\nis not definitionally equal to the right-hand type{indentExpr rhsTy}"
+  tryUnfold (goal : MVarId) (t : Expr) (err : MetaM MVarId) : MetaM MVarId := do
+    if let some t' ← unfoldDefinition? t then
+      liftReflToEqHEqCore goal t'
+    else
+      err
 
 /--
 Convert a goal of the form `x ~ y` into the form `x = y`, where `~` is a reflexive
 relation, that is, a relation which has a reflexive lemma tagged with the attribute `@[refl]`.
-If this can't be done, returns the original `MVarId`.
+
+Options:
+- If `failIfUnchanged = true` (default: `false`) then if this can't be done, returns the original `MVarId`.
+- If `allowHEq = true` (default: `false`) then allows converting the goal to `x ≍ y`.
 -/
-def _root_.Lean.MVarId.liftReflToEq (mvarId : MVarId) : MetaM MVarId := do
-  mvarId.checkNotAssigned `liftReflToEq
-  let .app (.app rel _) _ ← withReducible mvarId.getType' | return mvarId
-  if rel.isAppOf `Eq then
-    -- No need to lift Eq to Eq
-    return mvarId
-  for lem in ← (reflExt.getState (← getEnv)).getMatch rel do
-    let res ← observing? do
-      -- First create an equality relating the LHS and RHS
-      -- and reduce the goal to proving that LHS is related to LHS.
-      let [mvarIdEq, mvarIdR] ← mvarId.apply (← mkConstWithFreshMVarLevels ``rel_of_eq_and_refl)
-        | failure
-      -- Then fill in the proof of the latter by reflexivity.
-      let [] ← mvarIdR.apply (← mkConstWithFreshMVarLevels lem) | failure
-      return mvarIdEq
-    if let some mvarIdEq := res then
-      return mvarIdEq
-  return mvarId
+def _root_.Lean.MVarId.liftReflToEq (goal : MVarId) (allowHEq : Bool := false) (failIfUnchanged : Bool := false) : MetaM MVarId := do
+  goal.withContext do
+    goal.checkNotAssigned `liftReflToEq
+    let t ← goal.getType
+    if failIfUnchanged then
+      liftReflToEqHEqCore goal t allowHEq
+    else
+      return (← observing? (liftReflToEqHEqCore goal t allowHEq)).getD goal
 
 end Lean.Meta.Rfl
